src/variability.lean
@@ -1,110 +1,149 @@
-import data.set
 import data.finset
-
-import .SPL
-
-open SPL
 
 namespace variability
 
---constants {Feature : Type} 
---constants [t : fintype Feature] 
---constants [d : decidable_eq Feature]
---constants {L : SPL}
---parameters (L : SPL Feature)
- 
-constants {L : SPL}
+@[simp]
+def Config {Feature : Type} [fintype Feature] := finset Feature  
 
-section var 
+@[simp]
+def allConfigs {Feature : Type} [t1 : fintype Feature] : finset (finset Feature)
+    := finset.univ 
 
-inductive PC : Type
-| All
-| None
+inductive PC {Feature : Type} : Type
+| All  : PC 
+| None : PC
 | Atom : Feature → PC 
 | Not  : PC → PC
 | And  : PC → PC → PC
-| Or   : PC → PC → PC 
- 
-section PCSemantics
+| Or   : PC → PC → PC
 
-open PC
+open PC list 
 
---def allProducts := allConfigs Feature L
-#check @SPL 
-def semantics : PC → finset Config
-| All           := L.allConfigs
-| None          := ∅
-| (Atom f)      := L.allConfigs.filter (λ p, f ∈ p)
-| (Not pc)      := L.allConfigs.filter (λ p, p ∈ (semantics pc))
+def semantics {Feature : Type} [t : fintype Feature] [decidable_eq Feature]
+    : PC → finset (@Config Feature t)
+| (All)         := allConfigs
+| (None)        := ∅
+| (Atom f)      := allConfigs.filter (λ p, f ∈ p)
+| (Not pc)      := allConfigs.filter (λ p, p ∈ (semantics pc))
 | (And pc₁ pc₂) := (semantics pc₁) ∩ (semantics pc₂)
 | (Or  pc₁ pc₂) := (semantics pc₁) ∪ (semantics pc₂)
 
-end PCSemantics
+notation `⟦` p `⟧` := (semantics p)
 
-
-structure Var (α : Type) := (v : α) (pc : PC)
-
-structure Lifted (α : Type) := 
-    (s : list (Var α))
-    (disjoint : ∀ p q : Var α, p ∈ s ∧ q ∈ s ∧ p ≠ q → (semantics (PC.And p.pc q.pc)) = ∅)
-    (complete : semantics(list.foldr (PC.Or) (PC.None) (list.map (Var.pc) s)) = allProducts)
+structure Var {Feature: Type} [fintype Feature] (α : Type) := 
+    (v : α) (pc : @PC Feature)
 
 /-
-def set' (α : Type v) : Type v := α → PC
+def cover {Feature : Type} [t : fintype Feature] [d : decidable_eq Feature] {α : Type}
+    (v : list (@Var Feature t α)) : finset Config := 
+    semantics(foldr Or None (map Var.pc v))
 
-end var
-
-@[class]
-structure has_index (α : Type) {β : Type} :=
-(index_ : α → PC → β )
-
-def index (s : set' α) (pc : PC) : set α := (and pc) ∘ s
-
-instance : has_index (set' α) := --(set β):= 
-⟨variability.index⟩ 
-
-protected def mem (x : Var α) (s : set' α) : Prop := 
-    x.2 → (s x.1)
-
-instance : has_mem (Var α) (set' α) := ⟨variability.mem⟩
-
-protected def subset (s₁ s₂ : set' α) : Prop :=
-    ∀ a, a ∈ s₁ → a ∈ s₂
-
-instance : has_subset (set' α) := ⟨ variability.subset ⟩
-
-protected def sub {α : Type u} (s₁ s₂ : set' α) : set' α :=
-    λ (a : α), s₁ a ∧ ¬ (s₂ a)
-
-instance : has_sub (set' α) := ⟨ variability.sub ⟩
-
-protected def union (s₁ s₂ : set' α) : set' α :=
-    λ x, (s₁ x) ∨ (s₂ x)
-
-instance : has_union (set' α) :=
-⟨variability.union⟩
-
-def image (f : α → β) (s : set' α) : set' β :=
-λ x, (∀ y, f y = x ∧ s y)  
-
-infix `|`:90 := index
-
-variables (f  : set  α → set  β) (g  : set  β  → set  γ)
-variables (f' : set' α → set' β) (g' : set' β  → set' γ)
-theorem fun_comp_correct :
-    (∀ a ρ, (f (a | ρ) = (f' a) | ρ)) →
-    (∀ b ρ, (g (b | ρ) = (g' b) | ρ)) →
-    (∀ a ρ, (g ∘ f) (a | ρ) = ((g' ∘ f') a) | ρ) 
-    :=
-begin
-intros h₁ h₂ a ρ, simp, 
-rw h₁, rw← h₂ 
-end
+inductive disjointVars {Feature : Type} [t : fintype Feature] [d : decidable_eq Feature] {α : Type} : (list (@Var Feature t α)) → Prop
+| nil_disjoint : disjointVars [] 
+| cons_disjoint : ∀ (x : @Var Feature t α) (xs: list (@Var Feature t α)), ⟦x.pc⟧ ∩ cover xs = ∅ → disjointVars (x :: xs)
 -/
 
-end var
+def disjointPCs {Feature: Type} [t : fintype Feature] [decidable_eq Feature] {α : Type}
+    (s    : list (@Var Feature t α)) : Prop := 
+    ∀ (c : Config) (pc₁ pc₂ : PC), pc₁ ∈ map (Var.pc) s → pc₂ ∈ map (Var.pc) s → 
+                                           c ∈ ⟦pc₁⟧ → c ∈ ⟦pc₂⟧ → pc₁ = pc₂
 
-notation `⟦` p `⟧` := (semantics p)
+def completePCs {Feature: Type} [t : fintype Feature] [decidable_eq Feature] {α : Type} 
+    (s    : list (@Var Feature t α)) : Prop :=
+    ∀ (c : Config), ∃ (v : Var α), v ∈ s ∧ c ∈ ⟦v.pc⟧
+
+structure Lifted {Feature: Type} [t : fintype Feature] [decidable_eq Feature] {α : Type} :=
+    (s    : list (@Var Feature t α))
+    (disj : disjointPCs s) 
+    (comp : completePCs s)
+
 postfix `↑`:(max+1) := Lifted
+
+section 
+
+open classical
+
+lemma list_find {α : Type} (q : α → Prop) [decidable_pred q] : ∀ (l : list α), 
+                            (∃ y, y ∈ l ∧ q y) → (list.find q l).is_some := 
+begin
+    intros l h₁, --apply exists.elim h₁, intros a h₂, 
+    induction l,
+    -- base case
+    apply exists.elim h₁, intros a h₂, apply and.elim h₂, intros h₃ h₄, simp, 
+    apply not_mem_nil a h₃,
+    -- induction
+    unfold find, cases decidable.em (q l_hd) with hpos hneg,
+    { rw if_pos hpos, simp },
+    { rw if_neg hneg, apply exists.elim h₁, intros a h₂, apply l_ih, apply exists.intro a,
+      simp at h₂, rw and.comm at h₂, rw and_or_distrib_left at h₂, apply or.elim h₂, 
+      {intro h₃, apply and.elim h₃, intros h₄ h₅, rw← h₅ at hneg, contradiction},
+      {intro h₃, rw and.comm, exact h₃}
+    } 
+end
+
+end --section
+
+def index {Feature: Type} [t : fintype Feature] [d : decidable_eq Feature] {α : Type}
+    (v : @Lifted Feature t d α) (ρ : @Config Feature t) : α :=
+let pred := λ (u : @Var Feature t α) , ρ ∈ ⟦u.pc⟧,
+    e := find pred v.s,
+    p := (list_find pred v.s (v.comp ρ))
+in  (option.get p).v
+
+infix `|` := index
+
+/-
+def PCPartition {Feature: Type} [t : fintype Feature] [d: decidable_eq Feature] {α : Type} 
+    (v : @Lifted Feature t d α) : list (@PC Feature) := 
+    map (Var.pc) v.s
+-/
+
+def apply' {Feature : Type} [t: fintype Feature] [d: decidable_eq Feature] {α β : Type}
+    (f : @Lifted Feature t d (α → β)) (v : @Lifted Feature t d α) : list (@Var Feature t β) :=
+    let pairs := f.s.product v.s,
+        satPairs := filter (λ (p : ((@Var Feature t (α → β)) × Var α)) , ⟦p.1.pc⟧ ∩ ⟦p.2.pc⟧ ≠ ∅) pairs
+    in  map (λ (p : (Var (α → β) × Var α)), Var.mk (p.1.v p.2.v) (And p.1.pc p.2.pc)) satPairs
+
+lemma apply'_disjoint {Feature : Type} [t: fintype Feature] [d: decidable_eq Feature] {α β : Type} :
+    ∀ (f : @Lifted Feature t d (α → β)) (v : @Lifted Feature t d α), disjointPCs (apply' f v) := 
+begin
+    intros f v, unfold apply', simp, unfold disjointPCs, intros c pc₁ pc₂ h1 h2 h3 h4,
+    simp at h1, simp at h2, apply exists.elim h1, intros, apply exists.elim ᾰ, intros,
+    apply and.elim ᾰ_1, intros, apply and.elim ᾰ_2, intros, apply and.elim ᾰ_4, intros, 
+    apply exists.elim h2, intros, apply exists.elim ᾰ_8, intros,
+    apply and.elim ᾰ_9, intros, apply and.elim ᾰ_10, intros, apply and.elim ᾰ_12, intros,
+    rw← ᾰ_3 at h3, unfold semantics at h3, simp at h3, 
+    rw← ᾰ_11 at h4, unfold semantics at h4, simp at h4, 
+    rw← ᾰ_3, rw← ᾰ_11, have : a.pc = a_2.pc, 
+    apply f.disj, simp, existsi a, split, apply ᾰ_6, refl,
+    simp, existsi a_2, split, apply ᾰ_14, refl,
+    apply h3.left, apply h4.left,
+    rw this, have : a_1.pc = a_3.pc,
+    apply v.disj, simp, existsi a_1, split, apply ᾰ_7, refl, 
+    simp, existsi a_3, split, apply ᾰ_15, refl,   
+    apply exists.elim h1, intros a h5, apply exists.elim h5,
+    intros a_1 h6, apply and.elim h6, intros h7 h8, apply h3.right, apply h4.right,
+    rw this
+end
+
+lemma apply'_complete {Feature : Type} [t: fintype Feature] [d: decidable_eq Feature] {α β : Type} :
+    ∀ (f : @Lifted Feature t d (α → β)) (v : @Lifted Feature t d α), completePCs (apply' f v) := 
+begin
+    intros f v, unfold apply', simp, unfold completePCs, intros, simp, 
+    have : ∃ (v₁ : Var (α → β)), v₁ ∈ f.s ∧ c ∈ ⟦v₁.pc⟧, apply f.comp, apply exists.elim this, intros, 
+    have : ∃ (v₂ : Var α), v₂ ∈ v.s ∧ c ∈ ⟦v₂.pc⟧, apply v.comp, apply exists.elim this, intros,
+    existsi (Var.mk (a.v a_1.v) (a.pc.And a_1.pc)), simp, split, 
+    existsi a, existsi a_1, split, split, split, exact ᾰ.left, exact ᾰ_1.left,  
+    apply finset.ne_empty_of_mem, simp, split, apply ᾰ.right, apply ᾰ_1.right,
+    simp, unfold semantics, simp, split, apply ᾰ.right, apply ᾰ_1.right
+end
+
+def apply {Feature : Type} [t: fintype Feature] [d: decidable_eq Feature] {α β : Type}
+    (f : @Lifted Feature t d (α → β)) (v : @Lifted Feature t d α) : @Lifted Feature t d β :=
+⟨apply' f v, apply'_disjoint f v, apply'_complete f v⟩
+
+theorem apply_correct {Feature : Type} [t: fintype Feature] [d: decidable_eq Feature] (α β : Type) :
+    ∀ (f : @Lifted Feature t d (α → β)) (v : @Lifted Feature t d α) (ρ : @Config Feature t),
+    (apply f v) | ρ = (f | ρ) (v | ρ) :=
 
 end variability
